heap/top/ret_path0_verif.v
@@ -12,6 +12,16 @@ Include cprogs.heap.top.ret_path0.
 Theorem proof: functional_correctness_statement.
 Proof.
   cbv delta [functional_correctness_statement].
+  intros.
+  Intros.
+  (* forward. *)
+  sep_apply list_length; [lia |].
+  Intros.
+  forward.
+  unfold POSTCONDITION.
+  unfold abbreviate.
+  
+  forward.
 Admitted.
 
 End SH_Proof.
