heap/up/path0_verif.v
@@ -12,6 +12,11 @@ Include cprogs.heap.up.path0.
 Theorem proof: functional_correctness_statement.
 Proof.
   cbv delta [functional_correctness_statement].
+  intros.
+  Intros.
+  forward.
+  Exists Hl pos0 a' (Vint (IntRepr (pos0))).
+  entailer!.
 Admitted.
 
 End SH_Proof.
